ADTRefinement/Core.v
@@ -4,104 +4,90 @@ Generalizable All Variables.
 Set Implicit Arguments.
 
 Section MethodRefinement.
-  Variables oldRep newRep : Type.
-  (** Old and new representations **)
 
-  Variable SiR : oldRep -> newRep -> Prop.
+  (** Old and new representations **)
+  Variables oldRep newRep : Type.
+
   (** Simulation Relation *)
+  Variable SiR : oldRep -> newRep -> Prop.
 
   Notation "ro ≃ rn" := (SiR ro rn) (at level 70).
 
-  (** Refinement of a mutator method: the values of the computation
-      produced by applying a new mutator method [newMutator] to any new
+  (** Refinement of a constructor: the computation produced by
+   a constructor [newConstructor] should be a refinement
+   of the computation produced by the old constructor [oldObserver] on
+   [d].  That is, the following diagram should commute:
+<<
+           old constructor
+       Dom --------------> old rep
+        ∥                      |
+        ∥ id               SiR |
+        ∥                      |
+       Dom --------------> new rep
+          new constructor
+>>
+   *)
+
+  Definition refineConstructor
+             (Dom : Type)
+             (oldConstructor : constructorType oldRep Dom)
+             (newConstructor : constructorType newRep Dom)
+    := forall d,
+         refine (r_o' <- oldConstructor d;
+                 {r_n | r_o' ≃ r_n})
+                (newConstructor d).
+
+  (** Refinement of a method : the values of the computation
+      produced by applying a new method [newMethod] to any new
       state [r_n] related to an old state [r_o] by the simulation
       relation [SiR] are related by [SiR] to some value produced by
-      the corresponding old mutator on [r_o]. Related values
-      are taken to related values (with the new mutator potentially
+      the corresponding old method on [r_o]. Related values
+      are taken to related values (with the new method potentially
       producing more deterministic computations). That is, the
       following diagram commutes:
 <<
-                   old mutator
+                   old method
        old rep --------------> old rep
           |                         |
       SiR |                         | SiR
           ↓                         ↓
        new rep --------------> new rep
-                   new mutator
+                   new method
 >>  *)
 
-  Definition refineMutator
-             (Dom : Type)
-             (oldMutator : mutatorMethodType oldRep Dom)
-             (newMutator : mutatorMethodType newRep Dom)
-    := forall r_o r_n n, r_o ≃ r_n ->
-         refine (r_o' <- oldMutator r_o n;
-                 {r_n | r_o' ≃ r_n})
-                (newMutator r_n n).
-
-  (** Refinement of an observer method: the computation produced by
-   an observer [newObserver] on any new state [r_n] related to an old
-   state [r_o] by the simulation relation [SiR] should be a refinement
-   of the computation produced by the old observer [oldObserver] on
-   [r_n].  That is, the following diagram should commute:
-<<
-                  old observer
-       old rep --------------> ℕ
-          |                      ∥
-      SiR |                      ∥ id
-          ↓                      ∥
-       new rep --------------> ℕ
-                  new observer
->>
-   *)
-
-  Definition refineObserver
+  Definition refineMethod
              (Dom Cod : Type)
-             (oldObserver : observerMethodType oldRep Dom Cod)
-             (newObserver : observerMethodType newRep Dom Cod)
-    := forall r_o r_n n, r_o ≃ r_n ->
-         refine (oldObserver r_o n)
-                (newObserver r_n n).
+             (oldMethod : methodType oldRep Dom Cod)
+             (newMethod : methodType newRep Dom Cod)
+    := forall r_o r_n d, r_o ≃ r_n ->
+         refine (r_o' <- oldMethod r_o d;
+                 r_n' <- {r_n | fst r_o' ≃ r_n};
+                 ret (r_n', snd r_o'))
+                (newMethod r_n d).
 
 End MethodRefinement.
-
-Notation "c ↝ v" := (computes_to c v) (at level 70).
-
-(** We map from old indices to new indices because every method that
-    used to be callable should still be callable, and we don't care
-    about the other methods.  We place [refineADT] in [Type] so that
-    we can extract the simulation relation. *)
 
 Record refineADT {Sig} (A B : ADT Sig) :=
   refinesADT {
       SiR : _;
-      ADTRefinementPreservesMutators
-      : forall idx : MutatorIndex Sig,
-          @refineMutator
+      ADTRefinementPreservesConstructors
+      : forall idx : ConstructorIndex Sig,
+          @refineConstructor
             (Rep A) (Rep B) SiR
-            (MutatorDom Sig idx)
-            (MutatorMethods A idx)
-            (MutatorMethods B idx);
-      ADTRefinementPreservesObservers
-      : forall idx : ObserverIndex Sig,
-          @refineObserver
+            (ConstructorDom Sig idx)
+            (Constructors A idx)
+            (Constructors B idx);
+      ADTRefinementPreservesMethods
+      : forall idx : MethodIndex Sig,
+          @refineMethod
             (Rep A) (Rep B) SiR
-            (fst (ObserverDomCod Sig idx))
-            (snd (ObserverDomCod Sig idx))
-            (ObserverMethods A idx)
-            (ObserverMethods B idx) }.
-(** We should always just unfold [refineMutator] and [refineObserver]
+            (fst (MethodDomCod Sig idx))
+            (snd (MethodDomCod Sig idx))
+            (Methods A idx)
+            (Methods B idx) }.
+(** We should always just unfold [refineMethod] and [refineConstructor]
     into [refine], so that we can rewrite with lemmas about [refine]. *)
-Arguments refineMutator / .
-Arguments refineObserver / .
+Arguments refineMethod / .
+Arguments refineConstructor / .
 
 Notation "ro ≃ rn" := (@SiR _ _ _ _ ro rn) (at level 70).
-
-(*(** If our goal is a [Prop], then we can extract the simulation relation. *)
-Definition refineADT_SiR_elim {Sig} {A B : ADT Sig} (P : Prop)
-           (H : (Rep A -> Rep B -> Prop) -> P)
-           (H' : refineADT A B)
-: P
-  := match H' with
-       | refinesADT SiR _ _ => H SiR
-     end.*)
