ADTExamples/QueryStructure/Bookstore.v
@@ -1,6 +1,6 @@
 Require Import String Omega List FunctionalExtensionality Ensembles
         Computation ADT ADTRefinement ADTNotation QueryStructureSchema
-        BuildADTRefinements QueryQSSpecs InsertQSSpecs
+        BuildADTRefinements QueryQSSpecs InsertQSSpecs EmptyQSSpecs
         QueryStructure GeneralInsertRefinements ListInsertRefinements
         GeneralQueryRefinements ListQueryRefinements
         ProcessScheduler.AdditionalLemmas.
@@ -27,15 +27,15 @@ Section BookStoreExamples.
   Open Scope QSSchema.
 
   Definition BookStoreSchema :=
-    query structure schema
+    Query Structure Schema
       [ relation "Books" has
                 schema <"Author" :: string,
                         "Title" :: string,
                         "ISBN" :: nat>
                 where attributes ["Title"; "Author"] depend on ["ISBN"];
-        relation "Orders" has
+    relation "Orders" has
                 schema <"ISBN" :: nat,
-                        "Date" :: nat> ]
+    "Date" :: nat> ]
       enforcing [attribute "ISBN" of "Orders" references "Books"].
 
   Definition Books := GetRelationKey BookStoreSchema "Books".
@@ -68,37 +68,40 @@ Section BookStoreExamples.
    *)
 
   Local Open Scope ADTSig_scope.
-  Local Open Scope QueryStructureParsing_scope.
+  Local Open Scope QueryStructure_scope.
   Local Open Scope Schema.
   Local Open Scope QuerySpec.
   Local Open Scope string.
 
   Definition BookStoreSig : ADTSig :=
     ADTsignature {
-        "PlaceOrder" : rep × Order → rep,
-        "AddBook" : rep × Book → rep ;
-        "GetTitles" : rep × string → list string,
-        "NumOrders" : rep × string → nat
+        "InitBookstore" : unit → rep ,
+        "PlaceOrder" : rep × Order → rep × unit,
+        "AddBook" : rep × Book → rep × unit,
+        "GetTitles" : rep × string → rep × list string,
+        "NumOrders" : rep × string → rep × nat
       }.
 
   Definition BookStoreSpec : ADT BookStoreSig :=
-    QueryADTRep BookStoreRefRep {
+    QueryADTRep BookStoreSchema {
+      const "InitBookstore" (_ : unit) : rep := empty,
+
       (* [PlaceOrder] : Place an order into the 'Orders' table *)
-      def update "PlaceOrder" ( o : Order ) : rep :=
+      update "PlaceOrder" ( o : Order ) : unit :=
           Insert o into Orders,
 
       (* [AddBook] : Add a book to the inventory *)
-      def update "AddBook" ( b : Book ) : rep :=
-          Insert b into Books ;
+      update "AddBook" ( b : Book ) : unit :=
+          Insert b into Books ,
 
       (* [GetTitles] : The titles of books written by a given author *)
-      def query "GetTitles" ( author : string ) : list string :=
+      query "GetTitles" ( author : string ) : list string :=
         For (b in Books)
         Where (author = b!Author)
         Return (b!Title),
 
       (* [NumOrders] : The number of orders for a given author *)
-      def query "NumOrders" ( author : string ) : nat :=
+       query "NumOrders" ( author : string ) : nat :=
           Count (For (o in Orders) (b in Books)
                  Where (author = b!Author)
                  Where (b!ISBN = o!oISBN)
@@ -123,6 +126,17 @@ Section BookStoreExamples.
   eauto with typeclass_instances.
   Defined.
 
+  Lemma EnsembleListEquivalence_Empty :
+    forall qsSchema Ridx,
+      EnsembleListEquivalence
+        (GetUnConstrRelation (DropQSConstraints (QSEmptySpec qsSchema))
+                             Ridx) [].
+  Proof.
+    intros; rewrite GetRelDropConstraints; simpl; split; simpl; intros;
+    unfold GetRelation, In in *;
+    rewrite Build_EmptyRelation_IsEmpty in *; simpl in *; auto.
+  Qed.
+
   Definition BookStore :
     Sharpened BookStoreSpec.
   Proof.
@@ -133,26 +147,10 @@ Section BookStoreExamples.
       since ADT refinement preserves the simulation relation. *)
     hone representation using (@DropQSConstraints_SiR BookStoreSchema).
 
-    (* Step 2: Remove extraneous schema and cross-relation constraints
-       from the [PlaceOrder] mutator so that subsequent refinements
-       will only need to implement with the foreign key constraint. *)
-    hone mutator "PlaceOrder".
-    {
-      remove trivial insertion checks.
-      finish honing.
-    }
-
-    (* Step 3: Similarly remove extraneous schema and cross-relation
-       constraints from the [AddBook] mutator so that subsequent
-       refinements will only need to implement the single key
-       constraint. *)
-    hone mutator "AddBook".
-    {
-      remove trivial insertion checks.
-      remove_trivial_insertion_constraints r_n n Orders Books
-                                           oISBN ISBN H.
-      finish honing.
-    }
+    drop constraints from insert "PlaceOrder".
+    drop constraints from insert "AddBook".
+    drop constraints from query "GetTitles".
+    drop constraints from query "NumOrders".
 
     (* Step 4: Switch to an implementation of the representation
        type as a pair of lists of tuples. *)
@@ -160,36 +158,45 @@ Section BookStoreExamples.
 
     (* Step 5: Implement the [GetTitles] observer for the pair of lists
      representation. *)
-    hone observer "GetTitles".
+    hone method "GetTitles".
     {
       unfold BookStoreListImpl_SiR in *; split_and.
+      setoid_rewrite refineEquiv_pick_ex_computes_to_and.
+      simplify with monad laws.
       implement queries for lists.
+      setoid_rewrite refineEquiv_pick_pair_pair.
+      setoid_rewrite refineEquiv_pick_eq'.
+      repeat (rewrite refine_pick_val; [simplify with monad laws | eassumption]).
       finish honing.
     }
 
     (* Step 6: Implement the [NumOrders] observer for the pair of lists
      representation. *)
-    hone observer "NumOrders".
+    hone method "NumOrders".
     {
       unfold BookStoreListImpl_SiR in *; split_and.
-      unfold Count.
       (* We first swap the order of the 'fors' to make the
          implementation more efficient. *)
+      setoid_rewrite refineEquiv_pick_ex_computes_to_and.
+      simplify with monad laws.
       rewrite Equivalent_Swap_In.
       rewrite refine_Query_For_In_Equivalent;
         [ | apply Equivalent_Swap_In_Where with (qs := _)]; cbv beta.
       (* Now implement the list query. *)
       implement queries for lists.
+      setoid_rewrite refineEquiv_pick_pair_pair.
+      setoid_rewrite refineEquiv_pick_eq'.
+      repeat (rewrite refine_pick_val; [simplify with monad laws | eassumption]).
       rewrite map_length.
       finish honing.
     }
 
     (* Step 7: Implement the [AddBook] mutator for the pair of lists
      representation. *)
-    hone mutator "AddBook".
+    hone method "AddBook".
     {
-      unfold BookStoreListImpl_SiR in *; split_and.
       setoid_rewrite refineEquiv_split_ex.
+      unfold BookStoreListImpl_SiR in *; split_and.
       setoid_rewrite refineEquiv_pick_computes_to_and.
       simplify with monad laws.
       setoid_rewrite refine_unused_key_check
@@ -200,17 +207,19 @@ Section BookStoreExamples.
       with (attr_eq_dec' := ISBN_attr_dec)
              (attr_eq_dec := _); eauto.
       simplify with monad laws.
-      rewrite refine_pick_eq_ex_bind.
-      rewrite refineEquiv_pick_pair.
+      rewrite refine_pick_eq_ex_bind; simpl.
+      rewrite refineEquiv_pick_pair_pair.
+      setoid_rewrite refineEquiv_pick_eq'.
+      simplify with monad laws.
       Split Constraint Checks.
       implement insert for lists.
       unfold Orders, Books; congruence.
-      implement failed insert.
+      repeat (rewrite refine_pick_val; [rewrite refineEquiv_bind_unit | eassumption]); reflexivity.
     }
 
     (* Step 7: Implement the [PlaceOrder] mutator for the pair of lists
      representation. *)
-    hone mutator "PlaceOrder".
+    hone method "PlaceOrder".
     {
       unfold BookStoreListImpl_SiR in *; split_and.
       setoid_rewrite refineEquiv_split_ex.
@@ -219,14 +228,35 @@ Section BookStoreExamples.
                      (P_dec := _); eauto.
       simplify with monad laws.
       rewrite refine_pick_eq_ex_bind.
-      rewrite refineEquiv_pick_pair.
-      Split Constraint Checks.
-      implement insert for lists.
+      rewrite refineEquiv_pick_pair_pair.
+      setoid_rewrite refineEquiv_pick_eq'.
+      simplify with monad laws; simpl.
+      Split Constraint Checks; simpl.
+      setoid_rewrite ImplementListInsert_neq; eauto.
+      simplify with monad laws.
+      rewrite H;  setoid_rewrite ImplementListInsert_eq; eauto.
+      simplify with monad laws.
+      reflexivity.
       unfold Orders, Books; congruence.
-      implement failed insert.
+      rewrite H.
+      repeat (rewrite refine_pick_val; [rewrite refineEquiv_bind_unit | eassumption]); reflexivity.
     }
 
-    (* Step 8: Profit. :) *)
+    (* Step 8: Implement the [InitBookstore] constructor.*)
+    hone constructor "InitBookstore".
+    {
+      unfold BookStoreListImpl_SiR, DropQSConstraints_SiR.
+    repeat setoid_rewrite refineEquiv_pick_ex_computes_to_and.
+    repeat setoid_rewrite refineEquiv_pick_eq'.
+    simplify with monad laws.
+    rewrite refineEquiv_pick_pair.
+    repeat (rewrite refine_pick_val;
+            [simplify with monad laws
+             | apply EnsembleListEquivalence_Empty]).
+    subst_body; higher_order_1_reflexivity.
+    }
+
+    (* Step 9: Profit. :) *)
 
     finish sharpening.
   Defined.
