ADTExamples/QueryStructure/ProcessScheduler/ListBasedRefinement.v
@@ -1,11 +1,11 @@
-Require Import List Omega Ensembles.
-
-Require Import FMapAVL OrderedTypeEx.
-Require Import FMapExtensions.
-Require Import DBSchema SetEq AdditionalLemmas.
-Require Export ADTRefinement.BuildADTRefinements.
-Require Import GeneralInsertRefinements ListInsertRefinements
-        GeneralQueryRefinements ListQueryRefinements.
+Require Import String Omega List FunctionalExtensionality Ensembles
+        FMapAVL OrderedTypeEx FMapExtensions
+        Computation ADT ADTRefinement ADTNotation QueryStructureSchema
+        BuildADTRefinements QueryQSSpecs InsertQSSpecs EmptyQSSpecs
+        QueryStructure GeneralInsertRefinements ListInsertRefinements
+        GeneralQueryRefinements ListQueryRefinements
+        ProcessScheduler.AdditionalLemmas
+        DBSchema SetEq State.
 
 Unset Implicit Arguments.
 Notation "x '∈' y" := (In _ y x) (at level 50, no associativity).
@@ -84,62 +84,120 @@ Section ListBasedRefinement.
 
   Require Import Computation.Refinements.Tactics.
 
+  Lemma EnsembleListEquivalence_Empty :
+    forall qsSchema Ridx,
+      EnsembleListEquivalence
+        (GetUnConstrRelation (DropQSConstraints (QSEmptySpec qsSchema))
+                             Ridx) [].
+  Proof.
+    intros; rewrite GetRelDropConstraints; simpl; split; simpl; intros;
+    unfold GetRelation, In in *;
+    rewrite Build_EmptyRelation_IsEmpty in *; simpl in *; auto.
+  Qed.
+
   Definition ProcessScheduler :
     Sharpened ProcessSchedulerSpec.
   Proof.
     unfold ProcessSchedulerSpec.
 
     hone representation using (@DropQSConstraints_SiR ProcessSchedulerSchema).
-
-    hone mutator SPAWN.
-    {
-      unfold ForAll_In.
-      remove trivial insertion checks.
-      finish honing.
-    }
+    drop constraints from query ENUMERATE.
+    drop constraints from query GET_CPU_TIME.
+    unfold ForAll_In; drop constraints from insert SPAWN.
 
     (* == Introduce the list-based (SimpleDB) representation == *)
     hone representation using SimpleDB_equivalence.
 
+    Lemma refineEquiv_pick_and_and {A : Type} :
+      forall (PA PA' PA'' : Ensemble A),
+        refineEquiv {a | (PA a /\ PA' a) /\ PA'' a}
+                    {a | PA a /\ PA' a /\ PA'' a}.
+    Proof.
+      split; unfold refine; intros; inversion_by computes_to_inv;
+      repeat econstructor; eauto.
+    Qed.
+
     (* == Implement ENUMERATE == *)
-    hone observer ENUMERATE.
+    hone method ENUMERATE.
     {
-      unfold SimpleDB_equivalence in *.
+      unfold SimpleDB_equivalence in *; split_and.
+      setoid_rewrite refineEquiv_pick_ex_computes_to_and.
+      simplify with monad laws.
       implement queries for lists.
+      rewrite refineEquiv_pick_pair with
+      (PA := fun a => (forall a0 : Process, In a0 (snd a) -> fst a > a0 PID)
+                      /\ EnsembleListEquivalence (GetUnConstrRelation c PROCESSES) (snd a)).
+      rewrite refineEquiv_pick_pair_fst_dep with
+      (PA := fun a b => (forall a0 : Process, In a0 b -> a > a0 PID)).
+      repeat (rewrite refine_pick_val; [simplify with monad laws | eassumption]).
+      setoid_rewrite refineEquiv_pick_eq'.
+      simplify with monad laws.
       finish honing.
     }
 
     (* == Implement GET_CPU_TIME == *)
-    hone observer GET_CPU_TIME.
+    hone method GET_CPU_TIME.
     {
-      unfold SimpleDB_equivalence in *.
+      unfold SimpleDB_equivalence in *; split_and.
+      setoid_rewrite refineEquiv_pick_ex_computes_to_and.
+      simplify with monad laws.
       implement queries for lists.
+      rewrite refineEquiv_pick_pair with
+      (PA := fun a => (forall a0 : Process, In a0 (snd a) -> fst a > a0 PID)
+                      /\ EnsembleListEquivalence (GetUnConstrRelation c PROCESSES) (snd a)).
+      rewrite refineEquiv_pick_pair_fst_dep with
+      (PA := fun a b => (forall a0 : Process, In a0 b -> a > a0 PID)).
+      repeat (rewrite refine_pick_val; [simplify with monad laws | eassumption]).
+      setoid_rewrite refineEquiv_pick_eq'.
+      simplify with monad laws.
       finish honing.
     }
 
-    hone mutator SPAWN.
+    hone method SPAWN.
     {
       unfold SimpleDB_equivalence in *; split_and.
-       setoid_rewrite refineEquiv_split_ex.
-       setoid_rewrite refineEquiv_pick_computes_to_and.
-       setoid_rewrite (refine_pick_val _ (a := fst r_n)); eauto.
-       simplify with monad laws.
-       setoid_rewrite refine_decision; eauto; try simplify with monad laws.
-       setoid_rewrite refine_decision'; eauto; try simplify with monad laws.
-       rewrite refine_pick_eq_ex_bind.
-       rewrite refineEquiv_pick_pair_fst_dep with
-       (PA := fun (a : nat) (b : list Process) => forall t : Tuple, List.In t b -> a > t PID).
-       setoid_rewrite ImplementListInsert_eq; eauto;
-       simplify with monad laws.
-       setoid_rewrite (refine_pick_val _ (a := S (fst r_n))); eauto;
-       try simplify with monad laws.
-       finish honing.
-       simpl; intros; intuition.
-       subst; unfold BuildTuple, PID, ith_Bounded; simpl; omega.
-       generalize (H1 _ H3); omega.
-       intros; eapply H1; eapply H2; eauto.
-       intros; eapply H1; eapply H2; eauto.
-       intros; eapply H1; eapply H2; eauto.
+      setoid_rewrite refineEquiv_split_ex.
+      setoid_rewrite refineEquiv_pick_computes_to_and.
+      setoid_rewrite (refine_pick_val _ (a := fst r_n)); eauto.
+      simplify with monad laws.
+      setoid_rewrite refine_decision; eauto; try simplify with monad laws.
+      setoid_rewrite refine_decision'; eauto; try simplify with monad laws.
+      rewrite refine_pick_eq_ex_bind.
+      rewrite refineEquiv_pick_pair with
+      (PA := fun a => (forall a0 : Process, In a0 (snd a) -> fst a > a0 PID)
+                      /\ _ (snd a)).
+      rewrite refineEquiv_pick_pair_fst_dep with
+      (PA := fun (a : nat) (b : list Process) => forall t : Tuple, List.In t b -> a > t PID).
+      setoid_rewrite ImplementListInsert_eq; eauto;
+      simplify with monad laws.
+      setoid_rewrite (refine_pick_val _ (a := S (fst r_n))); eauto.
+      simplify with monad laws.
+      setoid_rewrite refineEquiv_pick_eq';
+        simplify with monad laws; simpl.
+      finish honing.
+      simpl; intros; intuition.
+      subst; unfold BuildTuple, PID, ith_Bounded; simpl; omega.
+      generalize (H1 _ H3); omega.
+      intros; eapply H1; eapply H2; eauto.
+      intros; eapply H1; eapply H2; eauto.
+      intros; eapply H1; eapply H2; eauto.
+    }
+
+    hone constructor INIT.
+    {
+      unfold SimpleDB_equivalence, DropQSConstraints_SiR.
+      repeat setoid_rewrite refineEquiv_pick_ex_computes_to_and.
+      repeat setoid_rewrite refineEquiv_pick_eq'.
+      simplify with monad laws.
+      rewrite refineEquiv_pick_pair_fst_dep with
+      (PA := fun a b => (forall a0 : Process, In a0 b -> a > a0 PID)).
+      repeat (rewrite refine_pick_val;
+              [simplify with monad laws
+              | apply EnsembleListEquivalence_Empty]).
+      rewrite refine_pick_val.
+      simplify with monad laws; 
+      subst_body; higher_order_1_reflexivity.
+      instantiate (1 := 0); simpl; intuition.
     }
 
     finish sharpening.
