ADTRefinement/GeneralRefinements.v
@@ -1,8 +1,5 @@
-Require Import Common Computation ADT Ensembles.
-Require Export ADTRefinement.Core ADTRefinement.SetoidMorphisms.
-
-Generalizable All Variables.
-Set Implicit Arguments.
+Require Import Common ADT.Core
+        ADTRefinement.Core ADTRefinement.SetoidMorphisms.
 
 (* To derive an ADT interactively from a specification [spec], we can
    build a dependent product [ {adt : _ & refineADT spec adt} ]. The
@@ -49,7 +46,7 @@ Tactic Notation "finish" "sharpening" := eexists; solve [ reflexivity | eapply r
 (* Honing tactic for refining the observer method with the specified index.
      This version of the tactic takes the new implementation as an argument. *)
 
-Tactic Notation "hone" "observer" constr(obsIdx) "using" constr(obsBody) :=
+Tactic Notation "hone'" "method" constr(obsIdx) "using" constr(obsBody) :=
     let A :=
         match goal with
             |- Sharpened ?A => constr:(A) end in
@@ -58,23 +55,23 @@ Tactic Notation "hone" "observer" constr(obsIdx) "using" constr(obsBody) :=
                 end in
     let mutIdx_eq' := fresh in
     let Rep' := eval simpl in (Rep A) in
-    let MutatorIndex' := eval simpl in (MutatorIndex ASig) in
-    let ObserverIndex' := eval simpl in (ObserverIndex ASig) in
-    let ObserverMethods' := eval simpl in (ObserverMethods A) in
-      assert (forall idx idx' : ObserverIndex', {idx = idx'} + {idx <> idx'})
+    let ConstructorIndex' := eval simpl in (ConstructorIndex ASig) in
+    let MethodIndex' := eval simpl in (MethodIndex ASig) in
+    let Methods' := eval simpl in (Methods A) in
+      assert (forall idx idx' : MethodIndex', {idx = idx'} + {idx <> idx'})
         as obsIdx_eq' by (decide equality);
       eapply SharpenStep;
-      [eapply (@refineADT_Build_ADT_Observer
+      [eapply (@refineADT_Build_ADT_Method
                  Rep' _ _ _
-                 (fun idx : ObserverIndex ASig => if (obsIdx_eq' idx ()) then
+                 (fun idx : MethodIndex ASig => if (obsIdx_eq' idx ()) then
                                obsBody
                              else
-                               ObserverMethods' idx))
+                               Methods' idx))
       | idtac]; cbv beta in *; simpl in *.
 
-  (* Honing tactic for refining the mutator method with the specified index.
+  (* Honing tactic for refining the constructor method with the specified index.
      This version of the tactic takes the new implementation as an argument. *)
-  Tactic Notation "hone" "mutator" constr(mutIdx) "using" constr(mutBody) :=
+  Tactic Notation "hone'" "constructor" constr(mutIdx) "using" constr(mutBody) :=
     let A :=
         match goal with
             |- Sharpened ?A => constr:(A) end in
@@ -83,18 +80,18 @@ Tactic Notation "hone" "observer" constr(obsIdx) "using" constr(obsBody) :=
                 end in
     let mutIdx_eq' := fresh in
     let Rep' := eval simpl in (Rep A) in
-    let MutatorIndex' := eval simpl in (MutatorIndex ASig) in
-    let ObserverIndex' := eval simpl in (ObserverIndex ASig) in
-    let MutatorMethods' := eval simpl in (MutatorMethods A) in
-      assert (forall idx idx' : MutatorIndex', {idx = idx'} + {idx <> idx'})
+    let ConstructorIndex' := eval simpl in (ConstructorIndex ASig) in
+    let MethodIndex' := eval simpl in (MethodIndex ASig) in
+    let Constructors' := eval simpl in (Constructors A) in
+      assert (forall idx idx' : ConstructorIndex', {idx = idx'} + {idx <> idx'})
         as mutIdx_eq' by (decide equality);
       eapply SharpenStep;
-        [eapply (@refineADT_Build_ADT_Mutators Rep'
+        [eapply (@refineADT_Build_ADT_Constructors Rep'
                    _
                    _
                    _
-                   (fun idx : MutatorIndex ASig => if (mutIdx_eq' idx mutIdx) then
+                   (fun idx : ConstructorIndex ASig => if (mutIdx_eq' idx mutIdx) then
                                  mutBody
                                else
-                                 MutatorMethods' idx))
+                                 Constructors' idx))
         | idtac]; cbv beta in *; simpl in *.
