ADTRefinement/Refinements/DelegateMethods.v
@@ -1,5 +1,7 @@
-Require Import Common Computation ADT Ensembles ADTRefinement.Core
-        ADTRefinement.GeneralRefinements Pick.
+Require Import Common Computation
+        ADT.ADTSig ADT.Core
+        ADTRefinement.Core ADTRefinement.GeneralRefinements
+        ADTRefinement.SetoidMorphisms.
 
 Section DelegateMethods.
 
@@ -16,32 +18,36 @@ Section DelegateMethods.
   (* ADT doing the delegating. *)
   Variable delegatorADT : ADT delegatorSig.
 
-
   (* Indices of the methods that will be delegated to. *)
   Variable delegateIndex : Type.
 
-  (* Domain and codomain of the new methods. *)
-  Variable delegateDomCod : delegateIndex -> Type * Type.
+  (* Codomain of the new methods. *)
+  Variable delegateCod : MethodIndex delegatorSig -> Type.
 
   (* Signature of the ADT being delegated to. *)
   Definition delegateSig :=
-    {| MutatorIndex := MutatorIndex delegatorSig;
-       ObserverIndex := delegateIndex;
-       MutatorDom := MutatorDom delegatorSig;
-       ObserverDomCod := delegateDomCod
+    {| ConstructorIndex := ConstructorIndex delegatorSig;
+       MethodIndex := MethodIndex delegatorSig;
+       ConstructorDom := ConstructorDom delegatorSig;
+       MethodDomCod idx :=
+         (fst (MethodDomCod delegatorSig idx), delegateCod idx)
     |}.
 
   (* ADT being delegated to. *)
   Variable delegateADT : ADT delegateSig.
 
+  Local Open Scope comp.
+
   Definition ADTwDelegatedMethods : ADT delegatorSig :=
     {| Rep := Rep delegatorADT * Rep delegateADT;
-       MutatorMethods idx r x :=
-         (r1 <- MutatorMethods delegatorADT idx (fst r) x;
-          r2 <- MutatorMethods delegateADT idx (snd r) x;
-          ret (r1, r2))%comp;
-       ObserverMethods idx r :=
-         ObserverMethods delegatorADT idx (fst r)
+       Constructors idx x :=
+         (r1 <- Constructors delegatorADT idx x;
+          r2 <- Constructors delegateADT idx x;
+          ret (r1, r2));
+       Methods idx r x :=
+         (r1 <- Methods delegatorADT idx (fst r) x;
+          r2 <- Methods delegateADT idx (snd r) x;
+          ret ((fst r1, fst r2), snd r1 ))
     |}.
 
   Lemma refineADT_DelegatedMethods :
@@ -52,80 +58,9 @@ Section DelegateMethods.
     (SiR := fun or nr => or = fst nr); simpl; intros; subst.
     - unfold refine; intros; inversion_by computes_to_inv; subst;
       econstructor; eauto.
-    - reflexivity.
+    - f_equiv; unfold pointwise_relation, refine; intros.
+      inversion_by computes_to_inv; subst;
+      repeat econstructor; eauto.
   Qed.
 
 End DelegateMethods.
-
-(*Section SwapDelegate.
-
-  (* Signature of the ADT doing the delegating. *)
-  Variable delegatorSig : ADTSig.
-  (* ADT doing the delegating. *)
-  Variable delegatorADT : ADT delegatorSig.
-
-
-  (* Indices of the methods that will be delegated to. *)
-  Variable delegateIndex : Type.
-  (* Domain and codomain of the new methods. *)
-  Variable delegateDomCod : delegateIndex -> Type * Type.
-
-
-  (* Reference ADT to delegate to. *)
-  Variable refDelegateADT : ADT (delegateSig delegatorSig delegateDomCod).
-  (* Implementation ADT to delegate to. *)
-  Variable implDelegateADT : ADT (delegateSig delegatorSig delegateDomCod).
-
-
-
-  (* The reference representation of the specification of the ADT
-     being delegated to. (A natural candidate is the representation of
-     [delegatorADT].) *)
-  Variable delegateRefRep : Type.
-
-  (* The specification of the mutators of the delegate ADT
-  specification. (If [delegateRefRep] is [delegatorADT], these are
-  simply specifications of the mutators of the latter. ) *)
-
-  Variable delegateMutatorSpecs :
-    forall idx,
-      mutatorMethodSpec delegateRefRep (MutatorDom delegateSig idx).
-
-  (* The specification of the mutators of the delegate ADT
-  specification. *)
-  Variable delegateObserverSpecs :
-    forall idx,
-      observerMethodSpec delegateRefRep
-                         (fst (ObserverDomCod delegateSig idx))
-                         (snd (ObserverDomCod delegateSig idx)).
-
-  (* The refinement assumes that [delegateADT] implements the above
-   spec. *)
-  Hypothesis refinesdelegateADTRefRep :
-    refineADT (pickImpl _ delegateMutatorSpecs delegateObserverSpecs)
-              delegateADT.
-
-  Definition SiR_refineADT {Sig}
-             {adt1 adt2 : ADT Sig}
-             (refines_adt1_adt2 : refineADT adt1 adt2)
-  : exists SiR : Rep adt1 -> Rep adt2 -> Prop,
-      forall idx : ObserverIndex Sig,
-        refineObserver SiR (ObserverMethods adt1 idx)
-                       (ObserverMethods adt2 idx).
-    destruct refines_adt1_adt2; eauto.
-  Defined.
-
-  Check (SiR_refineADT refinesdelegateADTRefRep).
-
-  Print ex_intro.
-
-  Lemma refinesDelegatedMethodPick :
-    forall (idx : delegateIndex)
-           (r : Rep delegateADT)
-           (x : (fst (ObserverDomCod delegateSig idx)))
-           (SiR' r' r ->
-       delegateObserverSpecs idx r' x c -> P c
-       end) ->
-      refine {c | P c} (ObserverMethods delegateADT idx r x).
-  Proof.
-    intros. *)
