ADTExamples/QueryStructure/Notations.v
@@ -1,6 +1,3 @@
-Reserved Infix ":"
-         (no associativity, at level 60).
-
 Reserved Notation "t ! r"
          (no associativity, at level 2,
           format "t ! r").
@@ -30,10 +27,10 @@ Reserved Notation "'schema' headings"
 Reserved Notation "'schema' headings 'where' constraints"
   (at level 0, headings at level 0, constraints at level 50).
 
-Reserved Notation "'query' 'structure' 'schema' relList "
+Reserved Notation "'Query' 'Structure' 'Schema' relList "
          (at level 0).
 
-Reserved Notation "'query' 'structure' 'schema' relList 'enforcing' constraints"
+Reserved Notation "'Query' 'Structure' 'Schema' relList 'enforcing' constraints"
          (at level 0, constraints at level 50).
 
 Reserved Notation "( x 'in' r ) bod"
